General formulization of the n-element version of the ring signature scheme

src/crypto_foundations/primitives/hash_function/hash_function.lean
@@ -2,24 +2,14 @@ import computational_complexity.complexity_class
 import crypto_foundations.dist_sem
 import computational_complexity.negligable
 
--- Extension of key type of the hash key to include the security_parameter
-def hash_key (K : Type) := ℕ × K
-
--- Extract the security parameter from the hash key
-def hash_key.sp {K : Type} : hash_key K → ℕ := λ k, k.1
-
--- Extract the actual key from the hash key
-def hash_key.key {K : Type} : hash_key K → K := λ k, k.2
-
 /-- `keygen` takes in a security parameter and outputs a key bundled with the parameter
   `hash` takes a `hash_key` from keygen and a string in the input space to a string in the output space -/
-structure hash_function (K : Type) (input_space output_space : ℕ → Type) :=
-(keygen (security_parameter : ℕ) : comp (hash_key K))
-(keygen_well_formed : ∀ n, (keygen n).is_well_formed)
-(keygen_correct : ∀ sp, (keygen sp).Pr_prop (λ k, k.sp = sp) = 1)
-(hash (s : hash_key K) (x : input_space s.sp) : output_space s.sp)
+structure hash_function (K : ℕ → Type) (input_space output_space : ℕ → Type) :=
+(keygen (sp : ℕ) : comp (K sp))
+(keygen_well_formed : ∀ sp, (keygen sp).is_well_formed)
+(hash {sp : ℕ} : K sp × input_space sp → output_space sp)
 
-variables {K : Type} {input_space output_space : ℕ → Type} [∀ n, decidable_eq (output_space n)]
+variables {K : ℕ → Type} {input_space output_space : ℕ → Type} [∀ n, decidable_eq (output_space n)]
 
 @[simp]
 instance hash_function.keygen.is_well_formed (H : hash_function K input_space output_space) (sp : ℕ) :
@@ -28,42 +18,28 @@ hash_function.keygen_well_formed H sp
 
 variable (H : hash_function K input_space output_space)
 
--- Because of correctness assumption, all elements in the support of keygen have matching security parameters
-lemma security_parameter_eq_of_mem_support_keygen (H : hash_function K input_space output_space)
-  (s : hash_key K) (n : ℕ) (hsn : s ∈ (H.keygen n).support) : s.sp = n :=
-begin
-  have := H.keygen_correct n,
-  rw comp.Pr_prop_eq_one_iff at this,
-  refine this s hsn,
-end
-
 /-- The security game for collision resistance as a probabalistic function. 
   Adversary implicitly recieves the secuirty parameter via the hashkey from `keygen`-/
 def collision_finding_experiment (H : hash_function K input_space output_space) 
-  (A : Π (s : hash_key K), comp ((input_space s.sp) × (input_space s.sp))) :
+  (A : Π (sp : ℕ) (k : K sp), comp ((input_space sp) × (input_space sp))) :
   ℕ → comp bool :=
-λ security_parameter,
-  comp.bind (H.keygen security_parameter) (λ s,
-  comp.bind (A s) (λ xs, comp.ret (H.hash s xs.1 = H.hash s xs.2)
+λ sp,
+  comp.bind (H.keygen sp) (λ k,
+  comp.bind (A sp k) (λ xs, comp.ret (H.hash (k, xs.1) = H.hash (k, xs.2))
 ))
 
-instance collision_finding_experiment.is_well_formed (H : hash_function K input_space output_space) 
-  (A : Π (s : hash_key K), comp ((input_space s.sp) × (input_space s.sp)))
-  (hA : ∀ (s : hash_key K), s ∈ (H.keygen s.sp).support → (A s).is_well_formed) 
-  (n : ℕ) : (collision_finding_experiment H A n).is_well_formed :=
-begin
-  simp [collision_finding_experiment],
-  refine λ s hs, hA s _,
-  exact (security_parameter_eq_of_mem_support_keygen H s n hs).symm ▸ hs
-end
+@[simp]
+lemma collision_finding_experiment.is_well_formed (H : hash_function K input_space output_space)
+  (A : Π (sp : ℕ) (k : K sp), comp ((input_space sp) × (input_space sp))) 
+  (sp : ℕ) : (collision_finding_experiment H A sp).is_well_formed ↔ 
+    (∀ (k : K sp), k ∈ (H.keygen sp).support → (A sp k).is_well_formed)  :=
+by simp [collision_finding_experiment]
 
-def negligable_expirement_success (exp : ℕ → comp bool) (h : ∀ n, (exp n).is_well_formed) : Prop :=
-negligable (λ n, comp.Pr (exp n))
+def negligable_expirement_success (exp : ℕ → comp bool) (h : ∀ sp, (exp sp).is_well_formed) : Prop :=
+negligable (λ sp, comp.Pr (exp sp))
 
--- TODO: look at poly-time requirements more closely
+-- TODO: Require A to be PPT
 def collision_resistant (H : hash_function K input_space output_space) : Prop :=
-∀ (A : Π (s : hash_key K), comp ((input_space s.sp) × (input_space s.sp)))
-  (hA : ∀ (b : hash_key K), b ∈ (H.keygen b.sp).support → (A b).is_well_formed)
-  (hA' : ∀ k, poly_time_comp (λ n, A (n, k))),
-negligable_expirement_success (collision_finding_experiment H A) 
-  (collision_finding_experiment.is_well_formed H A hA)
+∀ (A : Π (sp : ℕ) (k : K sp), comp ((input_space sp) × (input_space sp)))
+  (hA : ∀ (sp : ℕ) (k : K sp) , k ∈ (H.keygen sp).support → (A sp k).is_well_formed),
+negligable_expirement_success (collision_finding_experiment H A) (by simpa using hA)
