src/crypto_foundations/primitives/ring_signatures/hhs_ring_signature.lean
@@ -1,30 +1,66 @@
 import crypto_foundations.hardness_assumptions.hard_homogeneous_space
 import crypto_foundations.primitives.ring_signatures.ring_signature
+import crypto_foundations.primitives.hash_function.hash_function
+import data.vector2
 
 /-!
 # Hard Homogenous Space based Ring Signature Scheme
 -/
 
-variables (G X : ℕ → Type) [∀ n, fintype (G n)] [∀ n, fintype (X n)]
-  [∀ n, inhabited (X n)] [∀ n, decidable_eq (G n)] [∀ n, decidable_eq (X n)] 
-  [∀ n, homogeneous_space (G n) (X n)]
-
-variables (M S : Type)
+variables {M : Type} {S G X K : ℕ → Type}
+variables [∀ n, fintype (G n)] [∀ n, fintype (X n)] [∀ n, inhabited (X n)] 
+variables [∀ n, decidable_eq (G n)] [∀ n, decidable_eq (X n)] [∀ n, decidable_eq (K n)]
+variable [∀ n, homogeneous_space (G n) (X n)]
 
 /-- Construct a ring signature scheme from a hard homogenous space.
 `x₀` is an arbitrary generator in `X` used as a base for the public keys.
-TODO: clean this up so the simplifier can properly reduce things -/
-def hhs_ring_signature [hard_homogeneous_space G X] (x₀ : ∀ n, X n) : 
-  ring_signature_scheme M S G X :=
-λ n, {
-  generate_keys := comp.bind (comp.rnd (G n)) 
-    (λ g, comp.ret (g, g • x₀ n)),
-  generate_keys_well_formed := by simp,
-  sign := sorry,
-  sign_well_formed := sorry,
-  verify := sorry
+
+Given security parameter `sp`, a signature on `n` parties is an element
+  of type `K sp × vector (G sp) n × vector (G sp) n`.
+The first element is the hash key used to sign this, and the two vectors are the signature -/
+def ring_signature_scheme_of_hard_homogenous_space [hard_homogeneous_space G X] 
+  (x₀ : Π sp, X sp) (H : hash_function K (λ sp, list (X sp) × M) (λ sp, G sp)) : 
+  ring_signature M (λ sp n, K sp × vector (G sp) n × vector (G sp) n) X G :=
+{
+  gen := λ sp, comp.bind (comp.rnd (G sp)) 
+    (λ g, comp.ret (g • (x₀ sp), g)),
+  gen_well_formed := by apply_instance,
+  sign := begin
+    intros sp n i sk inp,
+    refine (comp.rnd (G sp)).bind (λ t₁, _),
+    refine (comp.rnd (vector (G sp) n)).bind (λ rs, _),
+    refine (comp.rnd (vector (G sp) n)).bind (λ cs, _),
+    let R := inp.1,
+    let m := inp.2,
+    let Ts : vector (X sp) n := vector.of_fn (λ j, (rs.nth j * cs.nth j) • R.nth j),
+    let Tᵢ : X sp := t₁ • (x₀ sp),
+    let Ts' : vector (X sp) n := vector.of_fn (λ j, if j = i then Tᵢ else Ts.nth j),
+    let h : list (X sp) × M := ⟨vector.to_list ((x₀ sp) ::ᵥ (R.append Ts')), m⟩,
+    refine (H.keygen sp).bind (λ k, _),
+    let c : G sp := H.hash (k, h),
+    let cᵢ : G sp := sorry,
+    let rᵢ : G sp := sorry,
+    let cs' : vector (G sp) n := vector.of_fn (λ j, if j = i then cᵢ else cs.nth j),
+    let rs' : vector (G sp) n := vector.of_fn (λ j, if j = i then rᵢ else rs.nth j),
+    refine comp.ret (k, cs', rs'),
+  end,
+  sign_well_formed := by apply_instance,
+  verify := begin
+    intros sp n inp,
+    let R : vector (X sp) n := inp.1,
+    let m : M := inp.2.1,
+    let k : K sp := inp.2.2.1,
+    let cs : vector (G sp) n := inp.2.2.2.1,
+    let rs : vector (G sp) n := inp.2.2.2.2,
+    let Ts : vector (X sp) n := vector.of_fn (λ j, (rs.nth j * cs.nth j) • R.nth j),
+    let h : list (X sp) × M := ⟨vector.to_list ((x₀ sp) ::ᵥ (R.append Ts)), m⟩,
+    exact H.hash (k, h) = cs.to_list.prod,
+  end
 }
 
-lemma hhs_ring_signature_complete [hard_homogeneous_space G X] (x₀ : ∀ n, X n) :
-  (hhs_ring_signature G X M S x₀).complete :=
+variables [hard_homogeneous_space G X] 
+  (x₀ : Π sp, X sp) (H : hash_function K (λ sp, list (X sp) × M) (λ sp, G sp))
+
+theorem hhs_ring_signature_complete :
+  (ring_signature_scheme_of_hard_homogenous_space x₀ H).complete :=
 sorry
